UnitTest/AttrParser.lean
@@ -164,6 +164,6 @@ macro "#assert " e:term : command =>
 #assert expectErrorType "!mod_arith.int<17 : x>" "integer type expected after ':' in modarith type"
 
 /-! ## Pointer type -/
-#assert expectSuccessType "!cuda_tile.ptr<i1>" (PointerType.mk (IntegerType.mk 1))
-#assert expectSuccessType "!cuda_tile.ptr<i32>" (PointerType.mk (IntegerType.mk 32))
+#assert expectSuccessType "!cuda_tile.ptr<i1>" (CudaTile.PointerType.mk (IntegerType.mk 1))
+#assert expectSuccessType "!cuda_tile.ptr<i32>" (CudaTile.PointerType.mk (IntegerType.mk 32))
 #assert expectErrorType "!cuda_tile.ptr<16>" "integer type expected"
